\begin{code}
module Type.BetaNBE.Completeness where
\end{code}

\begin{code}
open import Type
open import Type.Equality
open import Type.RenamingSubstitution
open import Type.BetaNormal
open import Type.BetaNBE
open import Type.BetaNormal.Equality

open import Relation.Binary.PropositionalEquality hiding (subst)
open import Data.Sum
open import Data.Empty
open import Data.Product
open import Function
\end{code}

\begin{code}
-- A Partial equivalence relation on values: 'equality' for values
-- It's also a Kripke Logical Relation

-- to get the completeness proof to go through we need an additional
-- property on function spaces called Unif(ormity).

CR : ∀{Φ} K → Val Φ K → Val Φ K → Set
CR *       n        n'        = n ≡ n'
CR (K ⇒ J) (inj₁ n) (inj₁ n') = n ≡ n' -- reify (inj₁ n) ≡ reify (inj₁ n')
CR (K ⇒ J) (inj₂ f) (inj₁ n') = ⊥
CR (K ⇒ J) (inj₁ n) (inj₂ f)  = ⊥
CR (K ⇒ J) (inj₂ f) (inj₂ f') =
  Unif f
  ×
  Unif f'
  ×
  ∀ {Ψ}
     → (ρ : Ren _ Ψ)
     → {v v' : Val Ψ K}
     → CR K v v'
       ---------------------------------------------------------
     → CR J (f ρ v) (f' ρ v')
  where
    -- Uniformity
    Unif : ∀{Φ K J} → (∀ {Ψ} → Ren Φ Ψ → Val Ψ K → Val Ψ J) → Set
    Unif {Φ}{K}{J} f = ∀{Ψ Ψ'}
      → (ρ : Ren Φ Ψ)
      → (ρ' : Ren Ψ Ψ')
      → (v v' : Val Ψ K)
      → CR K v v'
        --------—————————————————————————————————————————————————
      → CR J (renVal ρ' (f ρ v)) (f (ρ' ∘ ρ) (renVal ρ' v'))
\end{code}

CR is symmetric and transitive, it is not reflexive, but we if we
have a value that is related to something else by CR then we can
derive a reflexivity result for it.

\begin{code}
symCR : ∀{Φ K}{v v' : Val Φ K}
  → CR K v v'
    --------------------------
  → CR K v' v
symCR {K = *}                        p              = sym p
symCR {K = K ⇒ J} {inj₁ n} {inj₁ n'} p              = sym p
symCR {K = K ⇒ J} {inj₁ n} {inj₂ f'} ()
symCR {K = K ⇒ J} {inj₂ f} {inj₁ n'} ()
symCR {K = K ⇒ J} {inj₂ f} {inj₂ f'} (p , p' , p'') =
  p' , p , λ ρ q → symCR (p'' ρ (symCR q))

transCR : ∀{Φ K} {v v' v'' : Val Φ K}
  → CR K v v'
  → CR K v' v''
    ----------------------------------
  → CR K v v''
transCR {K = *}                                   p              q
  = trans p q
transCR {K = K ⇒ J} {inj₁ n} {inj₁ n'} {inj₁ n''} p              q
  = trans p q
transCR {K = K ⇒ J} {inj₁ n} {inj₁ n'} {inj₂ f''} p              ()
transCR {K = K ⇒ J} {inj₁ n} {inj₂ f'}            ()             q
transCR {K = K ⇒ J} {inj₂ f} {inj₁ n'}            ()             q
transCR {K = K ⇒ J} {inj₂ f} {inj₂ f'} {inj₁ n}   p              ()
transCR {K = K ⇒ J} {inj₂ f} {inj₂ f'} {inj₂ f''} (p , p' , p'') (q , q' , q'')
 = p , q' , λ ρ r → transCR (p'' ρ r) (q'' ρ (transCR (symCR r) r))

reflCR : ∀{Φ K}{v v' : Val Φ K}
  → CR K v v'
    ---------------------------
  → CR K v v
reflCR p = transCR p (symCR p)
\end{code}

reify takes two related values and produces to identical normal
forms. reflectCR works in the other direction for neutral terms. They
are not mutually defined in this version of NBE.

Composing reify with the fundamental theorem of CR defined later and
using reflectCR to build identify environments will give us the
completeness result.

\begin{code}
reflectCR : ∀{Φ K} → {n n' : Φ ⊢Ne⋆ K}
  → n ≡ n'
    -----------------------------
  → CR K (reflect n) (reflect n')
reflectCR {K = *}     p = cong ne p
reflectCR {K = K ⇒ J} p = p

reifyCR : ∀{Φ K} → {v v' : Val Φ K}
  → CR K v v'
    -------------------------------
  → reify v ≡ reify v'
reifyCR {K = *    }                    p              = p
reifyCR {K = K ⇒ J} {inj₁ n} {inj₁ n'} p              = cong ne p
reifyCR {K = K ⇒ J} {inj₁ n} {inj₂ f'} ()             
reifyCR {K = K ⇒ J} {inj₂ f} {inj₁ n'} ()             
reifyCR {K = K ⇒ J} {inj₂ f} {inj₂ f'} (p , p' , p'') =
  cong ƛ (reifyCR (p'' S (reflectCR refl)))
\end{code}

'equality' for environements/CR lifted from values to environements

\begin{code}
EnvCR : ∀ {Φ Ψ} → (η η' : Env Φ Ψ) →  Set
EnvCR η η' = ∀{K}(α : _ ∋⋆ K) → CR K (η α) (η' α) 
\end{code}

Closure under environment extension

\begin{code}
CR,,⋆ : ∀{Φ Ψ K}{η η' : Env Φ Ψ}
  → EnvCR η η'
  → {v v' : Val Ψ K}
  → CR K v v'
    ----------------------------
  → EnvCR (η ,,⋆ v) (η' ,,⋆ v')
CR,,⋆ p q Z     = q
CR,,⋆ p q (S α) = p α
\end{code}

Closure under application

\begin{code}
AppCR : ∀{Φ K J}
  → {f f' : Val Φ (K ⇒ J)}
  → CR (K ⇒ J) f f'
  → {v v' : Val Φ K}
  → CR K v v'
  → CR J (f ·V v) (f' ·V v')
AppCR {f = inj₁ n} {inj₁ n'} p              q =
  reflectCR (cong₂ _·_ p (reifyCR q))
AppCR {f = inj₁ n} {inj₂ f'} ()             q
AppCR {f = inj₂ f} {inj₁ n}  ()             q
AppCR {f = inj₂ f} {inj₂ f'} (p , p' , p'') q = p'' id q
\end{code}

renVal commutes with reflect

\begin{code}
renVal-reflect : ∀{Φ Ψ K}
  → (ρ : Ren Φ Ψ)
  → (n : Φ ⊢Ne⋆ K)
    --------------------------------------------------------
  → CR K (renVal ρ (reflect n)) (reflect (renNe ρ n))
renVal-reflect {K = *}     ρ n = refl
renVal-reflect {K = K ⇒ J} ρ n = renNe-cong (λ _ → refl) n
\end{code}

renaming commutes with reify

\begin{code}
ren-reify : ∀{K Φ Ψ}{v v' : Val Φ K}
  → CR K v v'
  → (ρ : Ren Φ Ψ)
    ---------------------------------------------
  → renNf ρ (reify v) ≡ reify (renVal ρ v')
ren-reify {*}                            p              ρ =
  cong (renNf ρ) p
ren-reify {K ⇒ J} {v = inj₁ n} {inj₁ n'} p              ρ =
  cong (ne ∘ renNe ρ) p
ren-reify {K ⇒ J} {v = inj₁ n} {inj₂ f'} ()             ρ
ren-reify {K ⇒ J} {v = inj₂ f} {inj₁ n'} ()             ρ
ren-reify {K ⇒ J} {v = inj₂ f} {inj₂ f'} (p , p' , p'') ρ = cong ƛ
  (trans (ren-reify (p'' S (reflectCR refl)) (ext ρ))
           (reifyCR ((transCR ( p' S (ext ρ) _ _ (reflectCR refl)) (AppCR {f = renVal (S ∘ ρ) (inj₂ f')}{renVal (S ∘ ρ) (inj₂ f')} ((λ ρ₁ ρ' v → p' (ρ₁ ∘ S ∘ ρ) ρ' v) , (λ ρ₁ ρ' v → p' (ρ₁ ∘ S ∘ ρ) ρ' v) ,  λ ρ' q → proj₂ (proj₂ (reflCR {v = inj₂ f'}{v' = inj₂ f} (symCR {v = inj₂ f}{v' = inj₂ f'}(p , p' , p'')))) (ρ' ∘ S ∘ ρ) q) (renVal-reflect (ext ρ) (` Z)))))))
\end{code}

first functor law for renVal

\begin{code}
renVal-id : ∀ {K Φ}{v v' : Val Φ K}
  → CR K v v'
    ------------------------
  → CR K (renVal id v) v'
renVal-id {*}                            p = trans (renNf-id _) p
renVal-id {K ⇒ J} {v = inj₁ n} {inj₁ n'} p = trans (renNe-id _) p
renVal-id {K ⇒ J} {v = inj₁ n} {inj₂ f'} ()
renVal-id {K ⇒ J} {v = inj₂ f} {inj₁ n'} () 
renVal-id {K ⇒ J} {v = inj₂ f} {inj₂ f'} p = p
\end{code}

second functor law for renVal

\begin{code}
renVal-comp : ∀ {K Φ Ψ Θ}
  → (ρ : Ren Φ Ψ)
  → (ρ' : Ren Ψ Θ)
  → {v v' : Val Φ K}
  → CR K v v'
  → CR K (renVal (ρ' ∘ ρ) v) (renVal ρ' (renVal ρ v'))
renVal-comp {*}      ρ ρ'                    p              =
  trans (cong (renNf (ρ' ∘ ρ)) p) (renNf-comp _)
renVal-comp {K ⇒ K₁} ρ ρ' {inj₁ n} {inj₁ n'} p              =
  trans (cong (renNe (ρ' ∘ ρ)) p) (renNe-comp _)
renVal-comp {K ⇒ K₁} ρ ρ' {inj₁ x} {inj₂ y} ()
renVal-comp {K ⇒ K₁} ρ ρ' {inj₂ y} {inj₁ x} ()
renVal-comp {K ⇒ K₁} ρ ρ' {inj₂ y} {inj₂ y₁} (p , p' , p'') =
  (λ ρ'' ρ''' v → p (ρ'' ∘ ρ' ∘ ρ) ρ''' v)
  ,
  (λ ρ'' ρ''' v → p' (ρ'' ∘ ρ' ∘ ρ) ρ''' v)
  ,
  λ ρ'' q → p'' (ρ'' ∘ ρ' ∘ ρ) q
\end{code}

CR is closed under renaming

\begin{code}
renCR : ∀{Φ Ψ K}{v v' : Val Φ K}
  → (ρ : Ren Φ Ψ)
  → CR K v v'
  → CR K (renVal ρ v) (renVal ρ v')
renCR {K = *}                        ρ p              = cong (renNf ρ) p
renCR {K = K ⇒ J} {inj₁ n} {inj₁ n'} ρ p              = cong (renNe ρ) p
renCR {K = K ⇒ J} {inj₁ n} {inj₂ f'} ρ ()
renCR {K = K ⇒ J} {inj₂ f} {inj₁ n'} ρ ()
renCR {K = K ⇒ J} {inj₂ f} {inj₂ f'} ρ (p , p' , p'') =
  (λ ρ' ρ'' v → p (ρ' ∘ ρ) ρ'' v)
  ,
  (λ ρ' ρ'' v → p' (ρ' ∘ ρ) ρ'' v)
  ,
  λ ρ' q → p'' (ρ' ∘ ρ) q
\end{code}

CR is closed under application
\begin{code}
renVal·V : ∀{K J Φ Ψ}
  → (ρ : Ren Φ Ψ)
  → {f f' : Val Φ (K ⇒ J)}
  → CR (K ⇒ J) f f'
  → {v v' : Val Φ K}
  → CR K v v'
    --------------------------------------------------------------
  → CR J (renVal ρ (f ·V v)) (renVal ρ f' ·V renVal ρ v')
renVal·V {J = *} ρ {inj₁ n} {inj₁ n'} p {v}{v'}  q =
  cong₂ (λ x y → ne (x · y)) (cong (renNe ρ) p) (ren-reify q ρ)
renVal·V {J = J ⇒ K} ρ {inj₁ n} {inj₁ n'} p      q = cong₂ _·_
  (cong (renNe ρ) p)
  (ren-reify q ρ)
renVal·V ρ {inj₁ n} {inj₂ f}  ()             q
renVal·V ρ {inj₂ f} {inj₁ n'} ()             q
renVal·V ρ {inj₂ f} {inj₂ f'} (p , p' , p'') q =
  transCR (p id ρ _ _ q) (p'' ρ (renCR ρ (reflCR (symCR q))))
\end{code}

identity extension lemma, (post) renaming commutes with eval, defined mutually

\begin{code}
idext : ∀{Φ Ψ K}{η η' : Env Φ Ψ}
  → EnvCR η η'
  → (t : Φ ⊢⋆ K)
    ----------------------------
  → CR K (eval t η) (eval t η')

renVal-eval : ∀{Φ Ψ Θ K}
  → (t : Ψ ⊢⋆ K)
  → {η η' : ∀{J} → Ψ ∋⋆ J → Val Φ J}
  → (p : EnvCR η η')
  → (ρ : Ren Φ Θ )
    ---------------------------------------------------------
  → CR K (renVal ρ (eval t η)) (eval t (renVal ρ ∘ η'))
  
idext p (` x)       = p x
idext p (Π B)     =
  cong Π (idext (CR,,⋆ (renCR S ∘ p) (reflectCR refl)) B)
idext p (A ⇒ B)     = cong₂ _⇒_ (idext p A) (idext p B)
idext p (ƛ B)     =
  (λ ρ ρ' v v' q →
    transCR (renVal-eval B (CR,,⋆ (renCR ρ ∘ reflCR ∘ p) q) ρ')
            (idext (λ { Z     → renCR ρ' (reflCR (symCR q))
                      ; (S x) → symCR (renVal-comp ρ ρ' (reflCR (p x)))})
                   B))
  ,
  (λ ρ ρ' v v' q →
    transCR
      (renVal-eval B (CR,,⋆ (renCR ρ ∘ reflCR ∘ symCR ∘ p) q) ρ')
      (idext (λ { Z  → renCR ρ' (reflCR (symCR q))
                ; (S x) → symCR (renVal-comp ρ ρ' (reflCR (symCR (p x))))})
             B)) -- first two terms are identical (except for symCR (p x))
  ,
  λ ρ q → idext (CR,,⋆ (renCR ρ ∘ p) q) B
idext p (A · B)     = AppCR (idext p A) (idext p B)
idext p μ1          = refl
idext p (con tcn)   = refl

renVal-eval (` x) p ρ = renCR ρ (p x)
renVal-eval (Π B) p ρ = cong Π (trans
    (renVal-eval B
                    (CR,,⋆ (renCR S ∘ p) (reflectCR refl))
                    (ext ρ))
    (idext (λ{ Z     → renVal-reflect (ext ρ) (` Z)
             ; (S x) → transCR
                  (symCR (renVal-comp S (ext ρ) (reflCR (symCR (p x)))))
                  (renVal-comp ρ S (reflCR (symCR (p x))))})
             B))
renVal-eval (A ⇒ B) p ρ =
  cong₂ _⇒_ (renVal-eval A p ρ) (renVal-eval B p ρ)
renVal-eval (ƛ B) {η}{η'} p ρ =
  (λ ρ' ρ'' v v' q →
    transCR (renVal-eval B (CR,,⋆ (renCR (ρ' ∘ ρ) ∘ p) q) ρ'')
            (idext (λ { Z     → renCR ρ'' (reflCR (symCR q))
                      ; (S x) → symCR (renVal-comp (ρ' ∘ ρ) ρ'' (p x))})
                   B))
  ,
  (λ ρ' ρ'' v v' q → transCR
    (renVal-eval
      B
      (CR,,⋆ (renCR ρ' ∘ renCR ρ ∘ reflCR ∘ symCR ∘ p) q) ρ'')
    (idext (λ { Z     → renCR ρ'' (reflCR (symCR q))
              ; (S x) → symCR
                  (renVal-comp ρ' ρ'' (renCR ρ (reflCR (symCR (p x)))))})
           B)) -- again two almost identical terms
  ,
  λ ρ' q → idext (λ { Z → q ; (S x) → renVal-comp ρ ρ' (p x) }) B
renVal-eval (A · B) p ρ = transCR
  (renVal·V ρ (idext (reflCR ∘ p) A) (idext (reflCR ∘ p) B))
  (AppCR (renVal-eval A p ρ) (renVal-eval B p ρ))
renVal-eval μ1          p ρ = refl
renVal-eval (con tcn)   p ρ = refl
\end{code}

(pre) renaming commutes with eval

\begin{code}
ren-eval : ∀{Φ Ψ Θ K}
  (t : Θ ⊢⋆ K)
  {η η' : ∀{J} → Ψ ∋⋆ J → Val Φ J}
  (p : EnvCR η η')
  (ρ : Ren Θ Ψ) →
  CR K (eval (ren ρ t) η) (eval t (η' ∘ ρ))
ren-eval (` x) p ρ = p (ρ x)
ren-eval (Π B) p ρ =
  cong Π (trans (ren-eval
                  B
                  (CR,,⋆ (renCR S ∘ p)
                          (reflectCR refl)) (ext ρ))
       (idext (λ{ Z     → reflectCR refl
                ; (S x) → (renCR S ∘ reflCR ∘ symCR ∘ p) (ρ x)}) B))
ren-eval (A ⇒ B) p ρ = cong₂ _⇒_ (ren-eval A p ρ) (ren-eval B p ρ) 
ren-eval (ƛ B) p ρ =
  (λ ρ' ρ'' v v' q → transCR
     (renVal-eval (ren (ext ρ) B) (CR,,⋆ (renCR ρ' ∘ reflCR ∘ p) q) ρ'')
     (idext (λ { Z → renCR ρ'' (reflCR (symCR q))
               ; (S x) → symCR (renVal-comp ρ' ρ'' (reflCR (p x)))})
            (ren (ext ρ) B)))
  ,
  (λ ρ' ρ'' v v' q → transCR
    (renVal-eval B (CR,,⋆ (renCR ρ' ∘ reflCR ∘ symCR ∘ p ∘ ρ) q) ρ'')
    (idext (λ { Z     →  renCR ρ'' (reflCR (symCR q))
              ; (S x) → symCR
                   (renVal-comp ρ' ρ'' (reflCR (symCR (p (ρ x)))))})
           B))
  ,
  λ ρ' q → transCR
    (ren-eval B (CR,,⋆ (renCR ρ' ∘ p) q) (ext ρ))
    (idext (λ { Z     → reflCR (symCR q)
              ; (S x) → renCR ρ' (reflCR (symCR (p (ρ x)))) }) B)
ren-eval (A · B) p ρ = AppCR (ren-eval A p ρ) (ren-eval B p ρ)
ren-eval μ1          p ρ = refl
ren-eval (con tcn)   p ρ = refl
\end{code}

Subsitution lemma

\begin{code}
subst-eval : ∀{Φ Ψ Θ K}
  (t : Θ ⊢⋆ K)
  {η η' : ∀{J} → Ψ ∋⋆ J → Val Φ J}
  (p : EnvCR η η')
  (σ : Sub Θ Ψ) →
  CR K (eval (subst σ t) η) (eval t (λ x → eval (σ x) η'))
subst-eval (` x)      p σ = idext p (σ x)
subst-eval (Π B)    p σ = cong Π (trans
  (subst-eval B (CR,,⋆ (renCR S ∘ p) (reflectCR refl)) (exts σ))
  (idext (λ{ Z     → reflectCR refl
           ; (S x) → transCR
                (ren-eval
                  (σ x)
                  (CR,,⋆ (renCR S ∘ reflCR ∘ symCR ∘ p) (reflectCR refl)) S)
                (symCR (renVal-eval (σ x)  (reflCR ∘ symCR ∘ p) S)) })
         B))
subst-eval (A ⇒ B)    p σ = cong₂ _⇒_ (subst-eval A p σ) (subst-eval B p σ)
subst-eval (ƛ B)      p σ =
  (λ ρ ρ' v v' q → transCR
     (renVal-eval (subst (exts σ) B) (CR,,⋆ (renCR ρ ∘ reflCR ∘ p) q) ρ')
     (idext (λ { Z     → renCR ρ' (reflCR (symCR q))
               ; (S x) → symCR (renVal-comp ρ ρ' (reflCR (p x)))})
            (subst (exts σ) B)))
  ,
  (λ ρ ρ' v v' q → transCR
    (renVal-eval B (CR,,⋆ (renCR ρ ∘ idext (reflCR ∘ symCR ∘ p) ∘ σ) q) ρ')
    (idext (λ { Z → renCR ρ' (reflCR (symCR q))
              ; (S x) → symCR
                   (renVal-comp ρ ρ' (idext (reflCR ∘ symCR ∘ p) (σ x)))})
           B))
  ,
  λ ρ q → transCR (subst-eval B (CR,,⋆ (renCR ρ ∘ p) q) (exts σ))
    (idext (λ { Z     → reflCR (symCR q)
              ; (S x) → transCR
                   (ren-eval
                     (σ x)
                     (CR,,⋆ (renCR ρ ∘ reflCR ∘ symCR ∘ p) (reflCR (symCR q)))
                     S)
                   (symCR (renVal-eval (σ x) (reflCR ∘ symCR ∘ p) ρ))})
           B)
subst-eval (A · B)    p σ = AppCR (subst-eval A p σ) (subst-eval B p σ)
subst-eval μ1          p ρ = refl
subst-eval (con tcn) p ρ   = refl
\end{code}

Fundamental Theorem of logical relations for CR

\begin{code}
fund : ∀{Φ Ψ K}{η η' : Env Φ Ψ}
  → EnvCR η η'
  → {t t' : Φ ⊢⋆ K}
  → t ≡β t' → CR K (eval t η) (eval t' η')
fund p (refl≡β A)          = idext p A
fund p (sym≡β q)           = symCR (fund (symCR ∘ p) q)
fund p (trans≡β q r)       = transCR (fund (reflCR ∘ p) q) (fund p r)
fund p (⇒≡β q r)           = cong₂ _⇒_ (fund p q) (fund p r)
fund p (Π≡β q)             =
  cong Π (fund (CR,,⋆ (renCR S ∘ p) (reflectCR refl)) q)
fund p (ƛ≡β {B = B}{B'} q) =
  (λ ρ ρ' v v' r → transCR
    (renVal-eval B (CR,,⋆ (renCR ρ ∘ reflCR ∘ p) r) ρ')
    (idext (λ { Z → renCR ρ' (reflCR (symCR r))
              ; (S x) → symCR (renVal-comp ρ ρ' (reflCR (p x)))})
           B))
  ,
  (λ ρ ρ' v v' r → transCR
     (renVal-eval B' (CR,,⋆ (renCR ρ ∘ reflCR ∘ symCR ∘ p) r) ρ')
     (idext (λ { Z → renCR ρ' (reflCR (symCR r))
               ; (S x) → symCR (renVal-comp ρ ρ' (reflCR (symCR (p x))))})
            B'))
  ,
  λ ρ r → fund (CR,,⋆ (renCR ρ ∘ p) r) q
fund p (·≡β q r) = AppCR (fund p q) (fund p r)
fund p (β≡β B A) =
  transCR (idext (λ { Z     → idext (reflCR ∘ p) A
                    ; (S x) → renVal-id (reflCR (p x))})
                 B)
          (symCR (subst-eval B (symCR ∘ p) (subst-cons ` A)))
\end{code}

constructing the identity CR

\begin{code}
idCR : ∀{Φ K} → (x : Φ ∋⋆ K) → CR K (idEnv Φ x) (idEnv Φ x)
idCR x = reflectCR refl
\end{code}

\begin{code}
completeness : ∀ {K Φ} {s t : Φ ⊢⋆ K} → s ≡β t → nf s ≡ nf t
completeness p = reifyCR (fund idCR p)
\end{code}
